PREFIX :        <http://www.ontologydesignpatterns.org/ont/dul/IOLite.owl#>
PREFIX DUL:     <http://www.ontologydesignpatterns.org/ont/dul/DUL.owl#>
PREFIX IOLite:  <http://www.ontologydesignpatterns.org/ont/dul/IOLite.owl#>
PREFIX owl:     <http://www.w3.org/2002/07/owl#>
PREFIX owl2xml: <http://www.w3.org/2006/12/owl2-xml#>
PREFIX rdf:     <http://www.w3.org/1999/02/22-rdf-syntax-ns#>
PREFIX rdfs:    <http://www.w3.org/2000/01/rdf-schema#>
PREFIX xsd:     <http://www.w3.org/2001/XMLSchema#>

owl:Thing  rdf:type  owl:Class .

IOLite:Writing  rdf:type  owl:Class;
        rdfs:comment     "An information realization based on conventional symbols.\nIt is a secondary code of communication (secondary means that it is about an original bodily expression, i.e. a primary code). Therefore, we are not considering here early forms of iconic expression, which could be considered primary.";
        rdfs:label       "Realizzazione scritta"@it , "Writing"@en;
        rdfs:subClassOf  IOLite:Depiction;
        rdfs:subClassOf  [ rdf:type            owl:Restriction;
                           owl:onProperty      DUL:realizes;
                           owl:someValuesFrom  IOLite:LinguisticObject
                         ] .

IOLite:Word  rdf:type    owl:Class;
        rdfs:comment     "A linguistic object consisting of a string (independently of its physical realization).\nIts topological unity can change according to its physical realization: as a written realization, its boundaries are blank spaces, as a spoken realization, sometimes is silence, sometimes not, and higher order features intervene.\nGrammatical notions, such as noun, verb, adjective, etc., are roles defined by a grammar, and words (or larger linguistic objects) can play those roles in a given language. E.g., the word 'share' can play both 'verb' and 'noun' roles in contemporary English, while the word 'come' can only play the 'verb' role in English, and the 'adverb' or 'conjunction' roles in Italian (but if we consider a word as only realized by phonemes, i.e. if we consider the oral realizations of 'come', there is no common word 'come' in the two languages).";
        rdfs:label       "Parola"@it , "Word"@en;
        rdfs:subClassOf  IOLite:LinguisticObject;
        rdfs:subClassOf  [ rdf:type           owl:Restriction;
                           owl:allValuesFrom  [ rdf:type          owl:Class;
                                                owl:complementOf  IOLite:Word
                                              ];
                           owl:onProperty     DUL:hasComponent
                         ] .

IOLite:WebPage  rdf:type  owl:Class;
        rdfs:label       "Web page"@en;
        rdfs:subClassOf  IOLite:MultimediaObject , IOLite:DigitalResource .

IOLite:Voicing  rdf:type  owl:Class;
        rdfs:comment     "An information realization consisting of uttered sounds. In natural agents, it always co-occurs with bodily movements.";
        rdfs:label       "Vocalizzazione"@it , "Voicing"@en;
        rdfs:subClassOf  IOLite:Sound;
        rdfs:subClassOf  [ rdf:type            owl:Restriction;
                           owl:onProperty      DUL:hasParticipant;
                           owl:someValuesFrom  DUL:PhysicalAgent
                         ] .

IOLite:Thesaurus  rdf:type  owl:Class;
        rdfs:comment     "A collection of categories organized according to a specified syntax, typically used to create a controlled terminology in a domain. A useful rdfs encoding of a typical thesaurus syntax is the SKOS schema.";
        rdfs:label       "Tesauro"@it , "Thesaurus"@en;
        rdfs:subClassOf  IOLite:KOS .

IOLite:Text  rdf:type    owl:Class;
        rdfs:comment     "A LinguisticObject composed of at least one Sentence, and assumed to be realized in written form.";
        rdfs:label       "Testo"@it , "Text"@en;
        rdfs:subClassOf  IOLite:LinguisticObject;
        rdfs:subClassOf  [ rdf:type            owl:Restriction;
                           owl:onProperty      DUL:hasComponent;
                           owl:someValuesFrom  IOLite:Sentence
                         ];
        rdfs:subClassOf  [ rdf:type            owl:Restriction;
                           owl:onProperty      DUL:isRealizedBy;
                           owl:someValuesFrom  IOLite:Writing
                         ] .

IOLite:Term  rdf:type    owl:Class;
        rdfs:comment     "A word or multiword that is established in some terminology from a domain of discourse.";
        rdfs:label       "Termine"@it , "Term"@en;
        rdfs:subClassOf  IOLite:LinguisticObject;
        rdfs:subClassOf  [ rdf:type            owl:Restriction;
                           owl:onProperty      IOLite:hasSchema;
                           owl:someValuesFrom  IOLite:KOS
                         ];
        rdfs:subClassOf  [ rdf:type     owl:Class;
                           owl:unionOf  ( IOLite:Multiword IOLite:Word )
                         ] .

IOLite:Statue  rdf:type  owl:Class;
        rdfs:comment     "wn noun: A sculpture representing a human or animal";
        rdfs:label       "Statua"@it , "Statue"@en;
        rdfs:subClassOf  IOLite:Sculpture .

IOLite:Speech  rdf:type  owl:Class;
        rdfs:comment     "Conventional sounds realizing explicit communication. Speech is a primary code of communication (primary means that is an original body expression, especially if first learnt).";
        rdfs:label       "Discorso"@it , "Speech"@en;
        rdfs:subClassOf  IOLite:Voicing , DUL:InformationRealization;
        rdfs:subClassOf  [ rdf:type            owl:Restriction;
                           owl:onProperty      DUL:realizes;
                           owl:someValuesFrom  IOLite:LinguisticObject
                         ] .

IOLite:Sound  rdf:type   owl:Class;
        rdfs:comment     "An information realization consisting of sound waves.";
        rdfs:label       "Sound"@en;
        rdfs:subClassOf  DUL:Process .

IOLite:Sentence  rdf:type  owl:Class;
        rdfs:comment     "A composition of Phrase(s), assumed to express a state of affairs (here modelled as a dul:Situation). Graphically, a period is usually considered its boundary.";
        rdfs:label       "Frase"@it , "Sentence"@en;
        rdfs:subClassOf  IOLite:LinguisticObject;
        rdfs:subClassOf  [ rdf:type            owl:Restriction;
                           owl:onProperty      DUL:expresses;
                           owl:someValuesFrom  DUL:Situation
                         ];
        rdfs:subClassOf  [ rdf:type            owl:Restriction;
                           owl:onProperty      DUL:hasComponent;
                           owl:someValuesFrom  IOLite:Phrase
                         ] .

IOLite:Sculpture  rdf:type  owl:Class;
        rdfs:comment     "wn noun: A three-dimensional work of plastic art";
        rdfs:label       "Scultura"@it , "Sculpture"@en;
        rdfs:subClassOf  IOLite:PlasticArt .

IOLite:PlasticArt  rdf:type  owl:Class;
        rdfs:comment     "wn noun: The arts of shaping or modeling; carving and sculpture";
        rdfs:label       "Opera plastica"@it , "Plastic art"@en;
        rdfs:subClassOf  IOLite:Depiction .

IOLite:Phrase  rdf:type  owl:Class;
        rdfs:comment     "A composition of Word(s) that can be considered a higher syntactic unit than a Word, and dul:isComponentOf a Sentence";
        rdfs:label       "Proposizione"@it , "Phrase"@en;
        rdfs:subClassOf  IOLite:LinguisticObject;
        rdfs:subClassOf  [ rdf:type            owl:Restriction;
                           owl:onProperty      DUL:isComponentOf;
                           owl:someValuesFrom  IOLite:Sentence
                         ];
        rdfs:subClassOf  [ rdf:type            owl:Restriction;
                           owl:onProperty      DUL:hasComponent;
                           owl:someValuesFrom  IOLite:Word
                         ] .

IOLite:Phoneme  rdf:type  owl:Class;
        rdfs:comment     "A part of a word as it can be realized by Voicing\nA written information realization can be 'about' a phoneme (as in the case of transcription systems), but it does not 'realize' it: only Grapheme(s) are realized by written information (Writing).\nA phoneme is not necessarily able to express a meaning (any dul:SocialObject), although it can in principle (e.g. 'a' in English).";
        rdfs:label       "Fonema"@it , "Phoneme"@en;
        rdfs:subClassOf  IOLite:LinguisticObject;
        rdfs:subClassOf  [ rdf:type           owl:Restriction;
                           owl:allValuesFrom  IOLite:Voicing;
                           owl:onProperty     DUL:isRealizedBy
                         ] .

IOLite:Painting  rdf:type  owl:Class;
        rdfs:comment     "wn noun: Graphic art consisting of an artistic composition made by applying paints to a surface; \"a small painting by Picasso\"; \"he bought the painting as an investment\"; \"his pictures hang in the Louvre\"";
        rdfs:label       "Dipinto"@it , "Painting"@en;
        rdfs:subClassOf  IOLite:GraphicArt .

IOLite:NaturalLanguage
        rdf:type         owl:Class;
        rdfs:comment     "A natural language, evolved and used in a community across time.\nNatural languages components are 'temporary' and 'reconstructed' out of actual usage. For example, a grammar for a (part of a) natural language has the status of a theory for that language, but alternative ones can exist (e.g. generative vs. construction grammars).";
        rdfs:label       "Linguaggio naturale"@it , "Natural language"@en;
        rdfs:subClassOf  IOLite:Language;
        rdfs:subClassOf  [ rdf:type            owl:Restriction;
                           owl:onProperty      DUL:isConceptualizedBy;
                           owl:someValuesFrom  DUL:Community
                         ] .

IOLite:Multiword  rdf:type  owl:Class;
        rdfs:comment     "A LinguisticObject made up of more than one Word, but distinct from a Phrase, which is a higher syntactic unit.";
        rdfs:label       "Lemma polirematico"@it , "Polyrhematic unit"@en;
        rdfs:subClassOf  IOLite:LinguisticObject;
        rdfs:subClassOf  [ rdf:type            owl:Restriction;
                           owl:minCardinality  "2"^^xsd:nonNegativeInteger;
                           owl:onProperty      DUL:hasComponent
                         ];
        rdfs:subClassOf  [ rdf:type            owl:Restriction;
                           owl:onProperty      DUL:hasComponent;
                           owl:someValuesFrom  IOLite:Word
                         ] .

IOLite:MultimediaObject
        rdf:type         owl:Class;
        rdfs:comment     "An information realization that realizes heterogeneous information objects. Examples include audiovisual performances, web pages, etc.";
        rdfs:label       "Oggetto multimediale"@it , "Multimedia object"@en;
        rdfs:subClassOf  DUL:InformationRealization;
        rdfs:subClassOf  [ rdf:type            owl:Restriction;
                           owl:minCardinality  "2"^^xsd:nonNegativeInteger;
                           owl:onProperty      DUL:realizes
                         ] .

IOLite:Morpheme  rdf:type  owl:Class;
        rdfs:comment     "A part of a word that can express a meaning, which is part of the meaning of the entire word.";
        rdfs:label       "Morfema"@it , "Morpheme"@en;
        rdfs:subClassOf  IOLite:LinguisticObject;
        rdfs:subClassOf  [ rdf:type            owl:Restriction;
                           owl:onProperty      DUL:expresses;
                           owl:someValuesFrom  [ rdf:type         owl:Restriction;
                                                 owl:cardinality  "1"^^xsd:nonNegativeInteger;
                                                 owl:onProperty   DUL:isComponentOf
                                               ]
                         ];
        rdfs:subClassOf  [ rdf:type            owl:Restriction;
                           owl:onProperty      DUL:isComponentOf;
                           owl:someValuesFrom  IOLite:Word
                         ] .

IOLite:LinguisticTheory
        rdf:type         owl:Class;
        rdfs:comment     "Any theory describing the structure and/or production and understanding of a natural language or a set of natural languages, or a component of one or more natural languages.";
        rdfs:label       "Teoria linguistica"@it , "Linguistic theory"@en;
        rdfs:subClassOf  DUL:Theory;
        rdfs:subClassOf  [ rdf:type            owl:Restriction;
                           owl:onProperty      DUL:describes;
                           owl:someValuesFrom  [ rdf:type            owl:Restriction;
                                                 owl:onProperty      DUL:isComponentOf;
                                                 owl:someValuesFrom  IOLite:NaturalLanguage
                                               ]
                         ] .

IOLite:LinguisticObject
        rdf:type         owl:Class;
        rdfs:comment     "An information object represented in a NaturalLanguage";
        rdfs:label       "Oggetto linguistico"@it , "Linguistic object"@en;
        rdfs:subClassOf  DUL:InformationObject;
        rdfs:subClassOf  [ rdf:type            owl:Restriction;
                           owl:onProperty      IOLite:hasRepresentationLanguage;
                           owl:someValuesFrom  IOLite:NaturalLanguage
                         ] .

IOLite:LinguisticFunction
        rdf:type         owl:Class;
        rdfs:comment     "Any linguistic function that classifies words according to a LinguisticTheory. \nThis class includes parts of speech, thematic roles, phrase structure components, verbal aspects, etc. e.g. Subject, Object, Instrument, Stative, etc.\nEach linguistic function must be defined in a LinguisticTheory; e.g. a thematic role can be defined either in a generative grammar, or in construction-based theory.";
        rdfs:label       "Funzione linguistica"@it , "Linguistic function"@en;
        rdfs:subClassOf  DUL:Role;
        rdfs:subClassOf  [ rdf:type            owl:Restriction;
                           owl:onProperty      DUL:isDefinedIn;
                           owl:someValuesFrom  IOLite:LinguisticTheory
                         ] .

IOLite:LinguisticAct  rdf:type  owl:Class;
        rdfs:comment     "A communicative situation including linguistic objects, agents, and a set of contexts: physical (informational realizations), conceptual (social objects), and referential (entities).\nA linguistic act has an associated CommunicativeFunction that it satisfies.";
        rdfs:label       "Atto linguistico"@it , "Linguistic act"@en;
        rdfs:subClassOf  DUL:PlanExecution;
        rdfs:subClassOf  [ rdf:type            owl:Restriction;
                           owl:onProperty      DUL:satisfies;
                           owl:someValuesFrom  IOLite:CommunicativeFunction
                         ];
        rdfs:subClassOf  [ rdf:type            owl:Restriction;
                           owl:onProperty      DUL:includesObject;
                           owl:someValuesFrom  DUL:SocialObject
                         ];
        rdfs:subClassOf  [ rdf:type            owl:Restriction;
                           owl:onProperty      DUL:includesObject;
                           owl:someValuesFrom  DUL:Agent
                         ];
        rdfs:subClassOf  [ rdf:type            owl:Restriction;
                           owl:onProperty      DUL:includesObject;
                           owl:someValuesFrom  IOLite:LinguisticObject
                         ];
        rdfs:subClassOf  [ rdf:type            owl:Restriction;
                           owl:onProperty      DUL:isSettingFor;
                           owl:someValuesFrom  DUL:InformationRealization
                         ];
        rdfs:subClassOf  [ rdf:type                     owl:Restriction;
                           owl:minQualifiedCardinality  "5"^^xsd:nonNegativeInteger;
                           owl:onClass                  DUL:Entity;
                           owl:onProperty               DUL:isSettingFor
                         ] .

IOLite:Lexicon  rdf:type  owl:Class;
        rdfs:comment     "A collection of lexical items (terms, entries, ...) that are witnessed to have a linguistic relevance.";
        rdfs:label       "Lessico"@it , "Lexicon"@en;
        rdfs:subClassOf  IOLite:KOS .

IOLite:Lexeme  rdf:type  owl:Class;
        rdfs:comment     "Lexical entries for dictionaries, lexica, etc. They are used to create reference forms of words.";
        rdfs:label       "Lessema"@it , "Lexeme"@en;
        rdfs:subClassOf  IOLite:Term;
        rdfs:subClassOf  [ rdf:type            owl:Restriction;
                           owl:onProperty      IOLite:hasSchema;
                           owl:someValuesFrom  IOLite:Lexicon
                         ];
        rdfs:subClassOf  [ rdf:type     owl:Class;
                           owl:unionOf  ( IOLite:Multiword IOLite:Word )
                         ] .

IOLite:Language  rdf:type  owl:Class;
        rdfs:comment     "A natural or artificial language, provided with an alphabet (or vocabulary) and combinatorial rules. In the case of natural languages, their components are 'temporary' and 'reconstructed' out of actual usage. For example, a grammar for a natural language has the status of a theory for that language, and alternative ones can exist (e.g. generative vs. construction grammars).\nAnother distinction, between the general (systemic) rules for a language, and the local (contextual) rules for e.g. a certain context, speaker, place, etc., can be made separately.\nThe most comprehensive classification of languages ha probably been made by Umberto Eco, based on the production modes of the 'signs' that are represented in a certain language. It uses several semiotic dimensions, and will be modeled in a forthcoming ontology.";
        rdfs:label       "Linguaggio"@it , "Language"@en;
        rdfs:subClassOf  DUL:Description .

IOLite:KOS  rdf:type     owl:Class;
        rdfs:comment     "Knowledge Organization Systems: thesauri, terminologies, classification schemes, subject hierarchies, etc.";
        rdfs:label       "Sistema di organizzazione della conoscenza"@it , "Knowledge organization system"@en;
        rdfs:subClassOf  IOLite:DataStructure .

IOLite:IconicObject  rdf:type  owl:Class;
        rdfs:comment     "An information object represented in an IconicLanguage";
        rdfs:label       "Oggetto iconico"@it , "Iconic object"@en;
        rdfs:subClassOf  DUL:InformationObject;
        rdfs:subClassOf  [ rdf:type            owl:Restriction;
                           owl:onProperty      IOLite:hasRepresentationLanguage;
                           owl:someValuesFrom  IOLite:IconicLanguage
                         ] .

IOLite:IconicLanguage
        rdf:type         owl:Class;
        rdfs:comment     "A language made up of graphical elements. It can be natural, artificial, and even formal.";
        rdfs:label       "Linguaggio iconico"@it , "Iconic language"@en;
        rdfs:subClassOf  IOLite:Language .

IOLite:GraphicArt  rdf:type  owl:Class;
        rdfs:comment     "wn noun: The arts of drawing or painting or printmaking";
        rdfs:label       "Opera grafica"@it , "Graphic art"@en;
        rdfs:subClassOf  IOLite:Depiction .

IOLite:Grapheme  rdf:type  owl:Class;
        rdfs:comment     "A part of a word as it can be realized by Writing\nA spoken information realization can be 'about' a grapheme (as in reading), but it does not 'realize' it. Only Phoneme(s) are realized by spoken information (Voicing).\nBTW, since spoken realizations are a 'primary' code of communication, the difference between direct and indirect spoken realizations (reading) should be considered relevant.\nA grapheme is not necessarily able to express a meaning (a dul:SocialObject), although it can in principle (e.g. 'a' in English).";
        rdfs:label       "Grafema"@it , "Grapheme"@en;
        rdfs:subClassOf  IOLite:LinguisticObject;
        rdfs:subClassOf  [ rdf:type           owl:Restriction;
                           owl:allValuesFrom  IOLite:Writing;
                           owl:onProperty     DUL:isRealizedBy
                         ] .

IOLite:Gesture  rdf:type  owl:Class;
        rdfs:label       "Gesto"@it , "Gesture"@en;
        rdfs:subClassOf  IOLite:BodilyMotion .

IOLite:FormalLanguage
        rdf:type         owl:Class;
        rdfs:comment     "A formal language, created by some human, with a fixed grammar, and usually with an explicit formal semantics (i.e. any FormalExpression that is a wff or a valid element of a FormalLanguage has an interpretation wrt to formal entities such as sets, categories, etc.).";
        rdfs:label       "Linguaggio formale"@it , "Formal language"@en;
        rdfs:subClassOf  IOLite:Language;
        rdfs:subClassOf  [ rdf:type           owl:Restriction;
                           owl:allValuesFrom  IOLite:FormalExpression;
                           owl:onProperty     DUL:hasPart
                         ] .

IOLite:FormalExpression
        rdf:type          owl:Class;
        rdfs:comment      "Any information object represented in a FormalLanguage, usually having a formal interpretation by a dul:FormalEntity, and used to formally represent any Entity";
        rdfs:label        "Espressione formale"@it , "Formal expression"@en;
        rdfs:subClassOf   DUL:InformationObject;
        rdfs:subClassOf   [ rdf:type            owl:Restriction;
                            owl:onProperty      IOLite:hasRepresentationLanguage;
                            owl:someValuesFrom  IOLite:FormalLanguage
                          ];
        rdfs:subClassOf   [ rdf:type            owl:Restriction;
                            owl:onProperty      IOLite:isFormalTermFor;
                            owl:someValuesFrom  DUL:InformationObject
                          ];
        owl:disjointWith  IOLite:KOS .

IOLite:Drawing  rdf:type  owl:Class;
        rdfs:comment     "wn noun: A representation of forms or objects on a surface by means of lines; \"drawings of abstract forms\"; \"he did complicated pen-and-ink drawings like medieval miniatures\"";
        rdfs:label       "Disegno"@it , "Drawing"@en;
        rdfs:subClassOf  IOLite:Depiction .

IOLite:DigitalResource
        rdf:type         owl:Class;
        rdfs:comment     "Any resource that can be computed, e.g. a file, a piece of (implemented) software. This assumes an encoding allowing the computation (e.g. html+http protocol).";
        rdfs:label       "Risorsa digitale"@it , "Digital resource"@en;
        rdfs:subClassOf  DUL:InformationRealization .

IOLite:DigitalPhoto  rdf:type  owl:Class;
        rdfs:label       "Digital photo"@en;
        rdfs:subClassOf  IOLite:DigitalResource .

IOLite:Depiction  rdf:type  owl:Class;
        rdfs:comment     "An information realization consisting of depicted images/signs of any sort (e.g. graffiti, drawings, inscriptions, pictures, sculptures, etc.), which are inscripted on a medium that lasts longer than the depicting act.\nIt also includes any early form of inscripted iconic expression, which can be considered as original bodily expressions.";
        rdfs:label       "Realizzazione visiva"@it , "Depiction"@en;
        rdfs:subClassOf  DUL:PhysicalArtifact , DUL:InformationRealization .

IOLite:Datum  rdf:type   owl:Class;
        rdfs:comment     "From WordNet: 'an item of factual information derived from measurement or research'";
        rdfs:label       "Dato"@it , "Datum"@en;
        rdfs:subClassOf  DUL:InformationObject .

IOLite:DataStructure  rdf:type  owl:Class;
        rdfs:comment     "Any data structure, including databases, schemas, lexica, knowledge organizations systems, etc.";
        rdfs:label       "Struttura di dati"@it , "Data structure"@en;
        rdfs:subClassOf  DUL:InformationObject;
        rdfs:subClassOf  [ rdf:type           owl:Restriction;
                           owl:allValuesFrom  IOLite:DigitalResource;
                           owl:onProperty     DUL:isRealizedBy
                         ] .

IOLite:DBSchema  rdf:type  owl:Class;
        rdfs:comment     "Any conceptual, logical or physical schema for a database.";
        rdfs:label       "Schema di base di dati"@it , "Database schema"@en;
        rdfs:subClassOf  IOLite:DataStructure .

IOLite:ContractText  rdf:type  owl:Class;
        rdfs:comment     "The text of a contract";
        rdfs:label       "Testo di un contratto"@it , "Contract text"@en;
        rdfs:subClassOf  IOLite:Text;
        rdfs:subClassOf  [ rdf:type            owl:Restriction;
                           owl:onProperty      DUL:expresses;
                           owl:someValuesFrom  DUL:Contract
                         ] .

IOLite:CommunicativeFunction
        rdf:type         owl:Class;
        rdfs:comment     "The functions, e.g. defined by Jakobson and by Buhler, which define types of linguistic acts. Jakobson's ones include referential, conative, expressive, phatic, metalinguistic, poetic. Each function has typical roles and tasks that must be played during a linguistic act that achieves the function.";
        rdfs:label       "Funzione comunicativa"@it , "Communicative function"@en;
        rdfs:subClassOf  DUL:Plan .

IOLite:Code  rdf:type    owl:Class;
        rdfs:comment     "Any piece of information expressing computational operations, objects, markup, etc.";
        rdfs:label       "Codice"@it , "Code"@en;
        rdfs:subClassOf  DUL:InformationObject;
        rdfs:subClassOf  [ rdf:type           owl:Restriction;
                           owl:allValuesFrom  IOLite:DigitalResource;
                           owl:onProperty     DUL:isRealizedBy
                         ] .

IOLite:BodilyMotion  rdf:type  owl:Class;
        rdfs:comment     "An information realization consisting of bodily movements.";
        rdfs:label       "Movimento corporeo"@it , "Bodily motion"@en;
        rdfs:subClassOf  DUL:InformationRealization , DUL:Action;
        rdfs:subClassOf  [ rdf:type            owl:Restriction;
                           owl:onProperty      DUL:hasParticipant;
                           owl:someValuesFrom  DUL:PhysicalAgent
                         ] .

DUL:Theory  rdf:type  owl:Class .

DUL:SocialObject  rdf:type  owl:Class .

DUL:Situation  rdf:type  owl:Class .

DUL:Role  rdf:type  owl:Class .

DUL:Process  rdf:type  owl:Class .

DUL:PlanExecution  rdf:type  owl:Class .

DUL:Plan  rdf:type  owl:Class .

DUL:PhysicalArtifact  rdf:type  owl:Class .

DUL:PhysicalAgent  rdf:type  owl:Class .

DUL:InformationRealization
        rdf:type  owl:Class .

DUL:InformationObject
        rdf:type  owl:Class .

DUL:InformationEntity
        rdf:type  owl:Class .

DUL:FormalEntity  rdf:type  owl:Class;
        rdfs:subClassOf  [ rdf:type           owl:Restriction;
                           owl:allValuesFrom  IOLite:FormalExpression;
                           owl:onProperty     IOLite:isAssignedTo
                         ] .

DUL:Entity  rdf:type  owl:Class .

DUL:Description  rdf:type  owl:Class .

DUL:Contract  rdf:type  owl:Class .

DUL:Community  rdf:type  owl:Class .

DUL:Agent  rdf:type  owl:Class .

DUL:Action  rdf:type  owl:Class .

IOLite:reuses  rdf:type     owl:ObjectProperty;
        rdfs:comment        "Any relation between information entities, where the first one reuses (includes, transforms, reengineers, etc.) the second one.";
        rdfs:domain         DUL:InformationEntity;
        rdfs:range          DUL:InformationEntity;
        rdfs:subPropertyOf  DUL:associatedWith;
        owl:inverseOf       IOLite:isReusedBy .

IOLite:reproduces  rdf:type  owl:ObjectProperty;
        rdfs:domain         DUL:InformationRealization;
        rdfs:label          "riproduce"@it , "reproduces"@en;
        rdfs:range          DUL:InformationRealization;
        rdfs:subPropertyOf  IOLite:encodes .

IOLite:metaphoricallyBlendsWith
        rdf:type            owl:SymmetricProperty , owl:ObjectProperty;
        rdfs:comment        "This property can be used to relate two social objects that are associated by means of a metaphorical blending, e.g. Greek and Aegyptian sphinges.";
        rdfs:domain         DUL:SocialObject;
        rdfs:label          "fusoMetaforicamenteCon"@it , "metaphorically blends with"@en;
        rdfs:range          DUL:SocialObject;
        rdfs:subPropertyOf  DUL:associatedWith;
        owl:inverseOf       IOLite:metaphoricallyBlendsWith .

IOLite:lexicalizes  rdf:type  owl:ObjectProperty;
        rdfs:comment        "A relation between linguistic objects and other information objects (including other linguistic objects).\nFor example, 'dog' can lexicalize a picture of a dog, a linguistic description of a dog, or the logical class: 'Dog'.\nThis relation is a subPropertyOf encodes .\nIn case of FormalExpression(s), it is not the inverse of isFormalTermFor: formal expressions can be said to 'be formal terms' for a LinguisticObject(s), while, independently, linguistic objects can be said to 'lexicalize' formal expressions. The difference is mainly pragmatic: one can take e.g. the word Dog, and decide to have a logical class 'Dog' for it. Someone else can see the logical class 'Dog', and decide to lexicalize it with the words dog, chien, cane, etc. While the relation seems similar, the pragmatic of using them is very different.";
        rdfs:domain         IOLite:LinguisticObject;
        rdfs:label          "lessicalizza"@it , "lexicalizes"@en;
        rdfs:range          DUL:InformationObject;
        rdfs:subPropertyOf  IOLite:encodes , DUL:expresses .

IOLite:isSchemaOf  rdf:type  owl:ObjectProperty;
        rdfs:comment        "A relation between social objects and schemata that organize them. For example, a Tag hasSchema a Folksonomy, a Lexeme hasSchema a Lexicon, etc.";
        rdfs:domain         IOLite:DataStructure;
        rdfs:label          "è schema di"@it , "is schema of"@en;
        rdfs:range          DUL:SocialObject;
        rdfs:subPropertyOf  DUL:associatedWith .

IOLite:isReusedBy  rdf:type  owl:ObjectProperty;
        rdfs:domain         DUL:InformationEntity;
        rdfs:range          DUL:InformationEntity;
        rdfs:subPropertyOf  DUL:associatedWith .

IOLite:isReproducedBy
        rdf:type            owl:ObjectProperty;
        rdfs:domain         DUL:InformationRealization;
        rdfs:label          "è riprodotto da"@it , "is reproduced by"@en;
        rdfs:range          DUL:InformationRealization;
        rdfs:subPropertyOf  IOLite:isEncodedBy;
        owl:inverseOf       IOLite:reproduces .

IOLite:isRepresentationLanguageOf
        rdf:type            owl:ObjectProperty;
        rdfs:domain         IOLite:Language;
        rdfs:label          "è il linguaggio di rappresentazione di"@it , "is representation language of"@en;
        rdfs:range          DUL:InformationEntity;
        rdfs:subPropertyOf  DUL:associatedWith;
        owl:inverseOf       IOLite:hasRepresentationLanguage .

IOLite:isOriginalOf  rdf:type  owl:ObjectProperty;
        rdfs:domain         DUL:InformationRealization;
        rdfs:label          "è l'originale di"@it , "is original of"@en;
        rdfs:range          DUL:InformationRealization;
        rdfs:subPropertyOf  DUL:associatedWith;
        owl:inverseOf       IOLite:isCopyOf .

IOLite:isLexicalizedBy
        rdf:type            owl:ObjectProperty;
        rdfs:comment        "A relation between linguistic objects and other information objects (including other linguistic objects).\nFor example, 'dog' can lexicalize a picture of a dog, a linguistic description of a dog, or the logical class: 'Dog'.\nThis relation is a subPropertyOf encodes .\nIn case of FormalExpression(s), it is not the inverse of isFormalTermFor: formal expressions can be said to 'be formal terms' for a LinguisticObject(s), while, independently, linguistic objects can be said to 'lexicalize' formal expressions. The difference is mainly pragmatic: one can take e.g. the word Dog, and decide to have a logical class 'Dog' for it. Someone else can see the logical class 'Dog', and decide to lexicalize it with the words dog, chien, cane, etc. While the relation seems similar, the pragmatic of using them is very different.";
        rdfs:domain         DUL:InformationObject;
        rdfs:label          "è lessicalizzato da"@it , "is lexicalized by"@en;
        rdfs:range          IOLite:LinguisticObject;
        rdfs:subPropertyOf  IOLite:isEncodedBy , DUL:isExpressedBy;
        owl:inverseOf       IOLite:lexicalizes .

IOLite:isGroundingFor
        rdf:type            owl:ObjectProperty;
        rdfs:domain         DUL:Entity;
        rdfs:label          "is grounding for"@en;
        rdfs:range          DUL:FormalEntity;
        rdfs:subPropertyOf  DUL:associatedWith .

IOLite:isFormallyRepresentedIn
        rdf:type            owl:ObjectProperty;
        rdfs:comment        "The relation between formal expressions, and anything that they are supposed to represent.\nE.g., 'the predicate 'MariachiInTijuana' formallyRepresents the dul:Collection of all mariachis in Tijuana'; 'the equivalence relation '<=>' formallyRepresents the concept of two entities having the same properties', 'the constant 'John' formallyRepresents the dul:NaturalPerson John.\nNotice that formal expressions are formally interpreted by instances of dul:FormalEntity";
        rdfs:domain         DUL:Entity;
        rdfs:label          "è rappresentato formalmente in"@it , "is formally represented in"@en;
        rdfs:range          IOLite:FormalExpression;
        rdfs:subPropertyOf  DUL:isReferenceOf;
        owl:inverseOf       IOLite:formallyRepresents .

IOLite:isFormalTermFor
        rdf:type            owl:ObjectProperty;
        rdfs:comment        "The relation between an InformationObject and a FormalExpression (constant, formula, term, sentence, proposition, axiom, etc.) that it is supposed to be given formal interpretation to formalize the InformationObject.\nNotice that FormalExpression(s) only are formal terms for InformationObject(s), not for Concept(s) or for other SocialObject(s). On their turn, information object can 'express' (see) SocialObject(s).\nE.g., the predicate (FormalExpression) 'TijuanaMariachi' isFormalTermFor the Term 'the mariachis in Tijuana' (that expresses the Collection of all mariachis in Tijuana); the Term 'equivalence relation' (that expresses the Concept of 'two entities having the same properties') hasFormalTerm the '<=>' symbol.";
        rdfs:domain         IOLite:FormalExpression;
        rdfs:label          "è termine formale per"@it , "is formal term for"@en;
        rdfs:range          DUL:InformationObject;
        rdfs:subPropertyOf  IOLite:encodes , DUL:expresses .

IOLite:isEncodedBy  rdf:type  owl:ObjectProperty;
        rdfs:comment        "Any relation between two information entities, with the first used as an alternative encoding of the second. This encoding can preserve all or part of the informational structure. For example, an XML encoding of a plain text file, a digital scanning of a physical paper document, a reproduction of a painting, etc.\nThe encoding can be so precise and close to the medium of realization, that distinguishing the maximally encoded object from its realization is superfluous (as in many cases of computer science information entities). For this reason, the relation holds for either dul:InformationObject(s) or dul:InformationRealization(s).\nSince the relation holds for either dul:InformationObject(s) or dul:InformationRealization(s), dul:realizes is a subproperty of it.";
        rdfs:subPropertyOf  DUL:associatedWith .

IOLite:isDigitallyReproducedBy
        rdf:type            owl:ObjectProperty;
        rdfs:domain         DUL:InformationRealization;
        rdfs:label          "è digitalmente riprodotto da"@it , "is digitally reproduced by"@en;
        rdfs:range          IOLite:DigitalResource;
        rdfs:subPropertyOf  IOLite:isReproducedBy;
        owl:inverseOf       IOLite:digitallyReproduces .

IOLite:isCulturalGroundingFor
        rdf:type            owl:ObjectProperty;
        rdfs:domain         DUL:SocialObject;
        rdfs:label          "è una sorgente culturale per"@it , "is cultural grounding for"@en;
        rdfs:range          DUL:SocialObject;
        rdfs:subPropertyOf  DUL:associatedWith .

IOLite:isCopyOf  rdf:type   owl:ObjectProperty;
        rdfs:comment        "The original information realization of some copy. Differently from reproductions, copies are not planned to have notable differences from the original. Master copies, author-signed paintings, etc. are examples of originals.";
        rdfs:domain         DUL:InformationRealization;
        rdfs:label          "è copia di"@it , "is copy of"@en;
        rdfs:range          DUL:InformationRealization;
        rdfs:subPropertyOf  DUL:associatedWith .

IOLite:isAuthorOf  rdf:type  owl:ObjectProperty;
        rdfs:domain         DUL:Agent;
        rdfs:label          "è autore di"@it , "is author of"@en;
        rdfs:range          DUL:InformationEntity;
        rdfs:subPropertyOf  DUL:associatedWith .

IOLite:isAssignmentOf
        rdf:type            owl:FunctionalProperty , owl:ObjectProperty;
        rdfs:comment        "The relation between a FormalExpression, and an Entity (a FormalEntity in case of classes, relations, etc.) that it is supposed to be the reference of the symbol (FormalExpression) that the Entity is an intepretation of. \nIn other words, this property expresses the 'formal interpretation' function, by which a logician 'assigns' an Entity to a FormalExpression. \nFor each type of formal expressions defined in a logical language, an assignment assumption should be indicated, for example, owl:Class should be restricted to: isAssignmentOf allValuesFrom Class. In addition, differently from the general relation formallyRepresents, isAssignmentOf is functional (and its inverse is inverse functional), in order to encode the Tarskian correspondence assumption.\nE.g., the Set of 'all mariachis in Tijuana' isAssignedTo the predicate (FormalExpression) 'TijuanaMariachi' (that isFormalTermFor a Term e.g. 'the mariachis in Tijuana').";
        rdfs:domain         IOLite:FormalExpression;
        rdfs:label          "è interpretata formalmente come"@it , "è assegnazione di"@it , "is formally interpreted as"@en;
        rdfs:range          DUL:Entity;
        rdfs:subPropertyOf  IOLite:formallyRepresents;
        owl:inverseOf       IOLite:isAssignedTo .

IOLite:isAssignedTo  rdf:type  owl:InverseFunctionalProperty , owl:ObjectProperty;
        rdfs:comment        "The relation between a FormalExpression, and an Entity (a FormalEntity in case of classes, relations, etc.) that it is supposed to be the reference of the symbol (FormalExpression) that the Entity is an intepretation of. \nIn other words, this is the 'formal interpretation' function, by which a logician 'assigns' an Entity to a FormalExpression.\nFor each type of formal expressions defined in a logical language, an assignment assumption should be indicated, for example, owl:Class should be restricted to: isAssignmentOf allValuesFrom Class. In addition, differently from the general relation formallyRepresents, isAssignmentOf is functional (and its inverse is inverse functional), in order to encode the Tarskian correspondence assumption.\nE.g., the Set of 'all mariachis in Tijuana' isAssignedTo the predicate (FormalExpression) 'TijuanaMariachi' (that isFormalTermFor a Term e.g. 'the mariachis in Tijuana').";
        rdfs:domain         DUL:Entity;
        rdfs:label          "è assegnata a"@it , "interpreta formalmente {@it}" , "formally interprets {@en}";
        rdfs:range          IOLite:FormalExpression;
        rdfs:subPropertyOf  IOLite:isFormallyRepresentedIn .

IOLite:hasSchema  rdf:type  owl:ObjectProperty;
        rdfs:comment        "A relation between social objects and schemata that organize them. For example, a Tag hasSchema a Folksonomy, a Lexeme hasSchema a Lexicon, etc.";
        rdfs:domain         DUL:SocialObject;
        rdfs:label          "ha schema"@it , "has schema"@en;
        rdfs:range          IOLite:DataStructure;
        rdfs:subPropertyOf  DUL:associatedWith;
        owl:inverseOf       IOLite:isSchemaOf .

IOLite:hasRepresentationLanguage
        rdf:type            owl:ObjectProperty;
        rdfs:domain         DUL:InformationEntity;
        rdfs:label          "ha linguaggio di rappresentazione"@it , "has representation language"@en;
        rdfs:range          IOLite:Language;
        rdfs:subPropertyOf  DUL:associatedWith .

IOLite:hasGrounding  rdf:type  owl:ObjectProperty;
        rdfs:comment        "A formal entity is grounded in some other entity when it is assumed as the (formal, extensional) interpretation of it, for example, the set Dog can be grounded in the collection of all actual dogs (or in some of them that the modeller intends).";
        rdfs:domain         DUL:FormalEntity;
        rdfs:label          "has grounding"@en;
        rdfs:range          DUL:Entity;
        rdfs:subPropertyOf  DUL:associatedWith;
        owl:inverseOf       IOLite:isGroundingFor .

IOLite:hasFormalTerm  rdf:type  owl:ObjectProperty;
        rdfs:comment        "The relation between an InformationObject and a FormalExpression (constant, formula, term, sentence, proposition, axiom, etc.) that it is supposed to be given formal interpretation to formalize the InformationObject.\nNotice that FormalExpression(s) only are formal terms for InformationObject(s), not for Concept(s) or other for SocialObject(s). On their turn, information object can 'express' (see) SocialObject(s).\nE.g., the predicate (FormalExpression) 'TijuanaMariachi' isFormalTermFor the Term 'the mariachis in Tijuana' (that expresses the Collection of all mariachis in Tijuana); the Term 'equivalence relation' (that expresses the Concept of 'two entities having the same properties') hasFormalTerm the '<=>' symbol.";
        rdfs:domain         DUL:InformationObject;
        rdfs:label          "ha termine formale"@it , "has formal term"@en;
        rdfs:range          IOLite:FormalExpression;
        rdfs:subPropertyOf  IOLite:isEncodedBy , DUL:isExpressedBy;
        owl:inverseOf       IOLite:isFormalTermFor .

IOLite:hasCulturalMixingWith
        rdf:type            owl:SymmetricProperty , owl:ObjectProperty;
        rdfs:domain         DUL:SocialObject;
        rdfs:label          "ha una fusione culturale con"@it , "has cultural mixing with"@en;
        rdfs:range          DUL:SocialObject;
        rdfs:subPropertyOf  DUL:associatedWith;
        owl:inverseOf       IOLite:hasCulturalMixingWith .

IOLite:hasCulturalGrounding
        rdf:type            owl:ObjectProperty;
        rdfs:domain         DUL:SocialObject;
        rdfs:label          "ha sorgente culturale"@it , "has cultural grounding"@en;
        rdfs:range          DUL:SocialObject;
        rdfs:subPropertyOf  DUL:associatedWith;
        owl:inverseOf       IOLite:isCulturalGroundingFor .

IOLite:hasAuthor  rdf:type  owl:ObjectProperty;
        rdfs:domain         DUL:InformationEntity;
        rdfs:label          "ha come autore"@it , "has author"@en;
        rdfs:range          DUL:Agent;
        rdfs:subPropertyOf  DUL:associatedWith;
        owl:inverseOf       IOLite:isAuthorOf .

IOLite:formallyRepresents
        rdf:type            owl:ObjectProperty;
        rdfs:comment        "The relation between formal expressions, and anything that they are supposed to represent.\nE.g., 'the predicate 'MariachiInTijuana' formallyRepresents the dul:Collection of all mariachis in Tijuana'; 'the equivalence relation '<=>' formallyRepresents the Concept of two entities having the same properties', 'the constant 'John' formallyRepresents the dul:NaturalPerson 'John'.\nNotice that a FormalExpression isAssignmentOf (is formally interpreted by) instances of dul:FormalEntity.\n\nformallyRepresents is a particular case of 'dul:isAbout', holding only for formal expressions. \nAnyway, a formal expression that  dul:expresses a dul:SocialObject is also possible, but treats formal expressions as any other kind of dul:InformationObject that express a 'social' or 'cognitive' semantics, not a formal one.";
        rdfs:domain         IOLite:FormalExpression;
        rdfs:label          "rappresenta formalmente"@it , "formally represents"@en;
        rdfs:range          DUL:Entity;
        rdfs:subPropertyOf  DUL:isAbout .

IOLite:encodes  rdf:type    owl:ObjectProperty;
        rdfs:comment        "Any relation between two information entities, with the first used as an alternative encoding of the second. This encoding can preserve all or part of the informational structure. For example, an XML encoding of a plain text file, a digital scanning of a physical paper document, a reproduction of a painting, etc.\nThe encoding can be so precise and close to the medium of realization, that distinguishing the maximally encoded object from its realization is superfluous (as in many cases of computer science information entities). For this reason, the relation holds for either dul:InformationObject(s) or dul:InformationRealization(s).\nSince the relation holds for either dul:InformationObject(s) or dul:InformationRealization(s), dul:realizes is a subproperty of it.";
        rdfs:domain         DUL:InformationEntity;
        rdfs:range          DUL:InformationEntity;
        rdfs:subPropertyOf  DUL:associatedWith;
        owl:inverseOf       IOLite:isEncodedBy .

IOLite:digitallyReproduces
        rdf:type            owl:ObjectProperty;
        rdfs:domain         IOLite:DigitalResource;
        rdfs:label          "riproduce digitalmente"@it , "digitally reproduces"@en;
        rdfs:range          DUL:InformationRealization;
        rdfs:subPropertyOf  IOLite:reproduces .

IOLite:combinatoriallyRelatedTo
        rdf:type            owl:SymmetricProperty , owl:ObjectProperty;
        rdfs:comment        "Any relation holding between two FormalExpression(s), e.g. a function over formal grammars, boolean operators, syntactic relations defined for the logical vocabulary of a formal language, etc.\nSyntactic relations from logical languages have a correspondance to some formal relation.";
        rdfs:domain         IOLite:FormalExpression;
        rdfs:range          IOLite:FormalExpression;
        rdfs:subPropertyOf  DUL:associatedWith;
        owl:inverseOf       IOLite:combinatoriallyRelatedTo .

DUL:satisfies  rdf:type  owl:ObjectProperty .

DUL:realizes  rdf:type      owl:ObjectProperty;
        rdfs:subPropertyOf  IOLite:encodes .

DUL:isSettingFor  rdf:type  owl:ObjectProperty .

DUL:isReferenceOf  rdf:type  owl:ObjectProperty .

DUL:isRealizedBy  rdf:type  owl:ObjectProperty;
        rdfs:subPropertyOf  IOLite:isEncodedBy .

DUL:isExpressedBy  rdf:type  owl:ObjectProperty .

DUL:isDefinedIn  rdf:type  owl:ObjectProperty .

DUL:isConceptualizedBy
        rdf:type  owl:ObjectProperty .

DUL:isComponentOf  rdf:type  owl:ObjectProperty .

DUL:isAbout  rdf:type  owl:ObjectProperty .

DUL:includesObject  rdf:type  owl:ObjectProperty .

DUL:hasParticipant  rdf:type  owl:ObjectProperty .

DUL:hasPart  rdf:type  owl:ObjectProperty .

DUL:hasComponent  rdf:type  owl:ObjectProperty .

DUL:expresses  rdf:type  owl:ObjectProperty .

DUL:describes  rdf:type  owl:ObjectProperty .

DUL:associatedWith  rdf:type  owl:ObjectProperty .

<http://www.ontologydesignpatterns.org/ont/dul/IOLite.owl>
        rdf:type         owl:Ontology;
        rdfs:comment     "An ontology of information objects, encodings and realizations, as a plugin to DOLCE-Ultralite (reusing mainly the dul:expresses and dul:realizes relations from it). \nSeveral patterns are contained inside this ontology:\n- encodings of information entities\n- kinds of realizations (gestural motions, depictions, digital, multimedia, speech, etc.)\n- combinatorial relations between information objects\n- relations between formal expressions and generalized expressions (lexicalizations, formalizations)\n- relations between formal expressions and their assignments in formal semantics\n- relations between information objects and schemata (data structures, KOS, etc.)\n- authorship\n- kinds of linguistic objects\n- copies, reproductions, etc.\n- cultural combination of information objects (reuse, mixing, metaphorical blending)";
        rdfs:label       "Information Objects ontology";
        owl:imports      <http://www.ontologydesignpatterns.org/ont/dul/DUL.owl>;
        owl:versionInfo  "In 1.8, all object properties have been aligned to associatedWith, and some comments have been added.\nIn 1.7, the encodes object property has been modified in order to support any kind of information entity (purely social object or realization), and to give justice to computer science pragmatic equivalence between information objects that are fully encoded for computing, and the actual bits travelling in a machine or network, based on that encoding. The realizes property has been consequenctly declared as a subproperty of encodes.\nAlso removed redundant owl:someValuesFrom axioms\nIn 1.6, broadened range of hasRepresentationLanguage\nIn 1.5, some fixes added wrt to new plugins (Roles.owl, CollectionsLite.owl).\nIn 1.4, all elements have got English labels. Added the class LinguisticAct, useful to relate Agent(s) when use information objects to express meaning with some CommunicativeFunction (from the theory by Jakobson). Moreover, the relation between formal patterns and information patterns have been enriched. Some bugs fixed." , "1.8" .
